replace AtomExhaustion2.v

src/FrameStack/Vulnerabilities/AtomExhaustion.v
@@ -1,81 +1,56 @@
-From CoreErlang.FrameStack Require SubstSemanticsLabeled.
+From CoreErlang.FrameStack Require Import SubstSemanticsLabeled.
+From stdpp Require Export gmap sets.
 
 Open Scope string_scope.
 
 Module AtomExhaustion.
 
-Import FrameStack.SubstSemanticsLabeled.
 Import ListNotations.
 
-Definition step_any_non_final (fs : FrameStack) (e : Redex) (fs' : FrameStack) (e' : Redex) : Prop :=
-  exists k, ⟨fs, e⟩ -[k]-> ⟨fs', e'⟩.
-Notation "⟨ fs , e ⟩ -->* ⟨ fs' , e' ⟩" := (step_any_non_final fs e fs' e').
 
+Inductive generates_at_least_n_unique_atoms :
+  FrameStack -> Redex -> gset string -> nat -> Prop :=
+| generates_terminal fs r s:
+  generates_at_least_n_unique_atoms fs r s 0
 
+| generates_step_false fs r l fs' r' s n:
+  ⟨ fs , r ⟩ -⌊ l ⌋-> ⟨ fs' , r' ⟩ ->
+  (generates_at_least_n_unique_atoms fs' r' s n) ->
+  generates_at_least_n_unique_atoms fs r s n
 
-Inductive atom_generating_cfg : FrameStack -> Redex -> Prop :=
-| list_to_atom_frame fs (vl : list Val) (v : Val) (vs' : ValSeq) (eff' : SideEffectList):
-  Some ((RValSeq vs'), eff') =
-    create_result (ICall (VLit "erlang") (VLit "list_to_atom")) (vl ++ [v]) ->
-  (atom_generating_cfg
-    (FParams (ICall (VLit "erlang") (VLit "list_to_atom")) vl [] :: fs)
-    (RValSeq [v])).
+| generates_step_true_not_unique fs r (av: string) fs' r' s n:
+  ⟨ fs , r ⟩ -⌊ Some (AtomCreation, [VLit (Atom av)]) ⌋-> ⟨ fs' , r' ⟩ ->
+  (generates_at_least_n_unique_atoms fs' r' s n) ->
+  generates_at_least_n_unique_atoms fs r s n
 
-
-Definition atom_generating_step (fs: FrameStack) (r: Redex) (fs': FrameStack) (r': Redex) : Prop :=
-  (atom_generating_cfg fs r) /\ ⟨ fs , r ⟩ --> ⟨ fs' , r' ⟩.
-
-
-Inductive generates_at_least_n_atoms : FrameStack -> Redex -> nat -> Prop :=
-| generates_0 fs r:
-  generates_at_least_n_atoms fs r 0
-
-| generates_n fs r n fs' r' fs'' r'':
-  ⟨ fs , r ⟩ -->* ⟨ fs' , r' ⟩ -> (atom_generating_cfg fs' r') ->
-  ⟨ fs' , r' ⟩ --> ⟨ fs'' , r'' ⟩ -> (generates_at_least_n_atoms fs'' r'' n) ->
-  generates_at_least_n_atoms fs r (S n).
-
-
-Inductive generates_at_least_n_atoms_three_way : FrameStack -> Redex -> nat -> Prop :=
-| generates_0_tw fs r:
-  generates_at_least_n_atoms_three_way fs r 0
-
-| generates_n_step_false fs r n fs' r':
-  ⟨ fs , r ⟩ --> ⟨ fs' , r' ⟩ -> (generates_at_least_n_atoms fs' r' n) ->
-  generates_at_least_n_atoms_three_way fs r n
-
-| generates_n_step_true fs r n fs' r':
-  (atom_generating_cfg fs r) ->
-  ⟨ fs , r ⟩ --> ⟨ fs' , r' ⟩ -> (generates_at_least_n_atoms fs' r' n) ->
-  generates_at_least_n_atoms_three_way fs r (S n).
-
+| generates_step_true_unique fs r (av: string) fs' r' s n:
+  ⟨ fs , r ⟩ -⌊ Some (AtomCreation, [VLit (Atom av)]) ⌋-> ⟨ fs' , r' ⟩ ->
+  av ∉ s ->
+  (generates_at_least_n_unique_atoms fs' r' ({[av]} ∪ s) n) ->
+  generates_at_least_n_unique_atoms fs r s (S n).
 
 Definition call_of_list_to_atom: Exp :=
   ECall (˝VLit "erlang") (˝VLit "list_to_atom")
     [˝VCons (VLit 104%Z) (VCons (VLit 101%Z) (VCons (VLit 108%Z) (VCons (VLit 108%Z) (VCons (VLit 111%Z) (VNil)))))].
 
-Ltac do_step := econstructor; [constructor; auto|simpl].
+Ltac apply_proper_constr := 
+  eapply generates_terminal || (
+  eapply generates_step_true_unique;
+    [econstructor; reflexivity
+    |set_solver 
+    |] || (
+  eapply generates_step_true_not_unique;
+    [econstructor; reflexivity
+    |] ||
+  eapply generates_step_false;
+    [econstructor; try (scope_solver || congruence)
+    |simpl]
+)).
 
-Goal generates_at_least_n_atoms [] call_of_list_to_atom 1.
+Goal generates_at_least_n_unique_atoms [] call_of_list_to_atom ∅ 1.
 Proof.
-  econstructor.
-  1: {
-    unfold call_of_list_to_atom, step_any_non_final. eexists.
-    do 6 do_step. congruence. do_step. scope_solver. apply step_refl.
-  }
-  all: econstructor; reflexivity.
-Qed.
-
-Lemma generates_at_least_n_atoms_rec:
-  forall n fs r, generates_at_least_n_atoms fs r (S n) -> generates_at_least_n_atoms fs r n.
-Proof.
-  induction n.
-  - econstructor.
-  - intros. inv H. econstructor.
-    + exact H1.
-    + exact H2.
-    + exact H3.
-    + specialize (IHn _ _ H6). exact IHn.
+  unfold call_of_list_to_atom.
+  repeat apply_proper_constr.
 Qed.
 
 Definition infinite_atom_g (e : Exp) : Exp :=
@@ -88,42 +63,17 @@ Definition infinite_atom_g (e : Exp) : Exp :=
                 (EApp (˝VFunId (2, 1)) [˝VVar 0]))))]
     (EApp (˝VFunId (0, 1)) [e]).
 
-Goal forall n fs x,
-  generates_at_least_n_atoms fs (infinite_atom_g (˝VLit (Integer x))) n.
+Goal generates_at_least_n_unique_atoms [] (infinite_atom_g (˝VLit (Integer 0))) ∅ 20.
 Proof.
-  induction n.
-  - econstructor.
-  - intros. econstructor.
-    + unfold step_any_non_final. eexists.
-      unfold infinite_atom_g.
-      do 3 do_step. scope_solver. do 2 do_step. congruence.
-      do_step. eapply step_trans. eapply eval_cool_params. reflexivity. simpl.
-      do 10 do_step. congruence. do_step. econstructor.
-    + econstructor. reflexivity.
-    + eapply eval_cool_params. reflexivity.
-    + simpl. unfold eval_list_atom. simpl. clear IHn. revert fs x. induction n. 
-      * econstructor.
-      * intros. econstructor.
-        -- unfold step_any_non_final. eexists.
-           do 8 do_step. congruence. do 3 do_step.
-           eapply step_trans. eapply eval_cool_params. reflexivity.
-           unfold eval_arith. simpl. do 3 do_step. scope_solver.
-           do 2 do_step. congruence. do_step.
-           eapply step_trans. eapply eval_cool_params. reflexivity. simpl.
-           do 10 do_step. congruence. do_step. econstructor.
-        -- econstructor. reflexivity.
-        -- eapply eval_cool_params. reflexivity.
-        -- specialize (IHn fs (x + 1)%Z). assumption.
+  unfold infinite_atom_g.
+  do 19 (apply_proper_constr; [reflexivity|simpl];
+  do 6 apply_proper_constr; [reflexivity|simpl];
+  do 3 apply_proper_constr; [reflexivity|simpl];
+  do 21 apply_proper_constr; [reflexivity|simpl]).
+  apply_proper_constr; [reflexivity|simpl].
+  do 6 apply_proper_constr; [reflexivity|simpl].
+  do 3 apply_proper_constr; [reflexivity|simpl].
+  do 10 apply_proper_constr.
 Qed.
-
-(* Goal forall n fs x,
-  generates_at_least_n_atoms_three_way fs (infinite_atom_g (˝VLit (Integer x))) n.
-Proof.
-  induction n.
-  - econstructor.
-  - intros. unfold infinite_atom_g. eapply *)
-
-(* Construct smart tactics *)
-(* how to define tactics *)
 
 End AtomExhaustion.
